---
target-deck: CSARCH1::Boolean identities
tags: [CSARCH1]
title: Boolean identities
---

## Boolean identities
<!--ID: 1738378824080-->

### $X \cdot 0$

$X \cdot 0 = 0$, by **operations with 0 & 1**
<!--ID: 1738378824087-->

### $X + 1$

$X + 1 = 1$, by **operations with 0 & 1**
<!--ID: 1738378824089-->

### $X \cdot 1$

$X \cdot 1 = X$, by **operations with 0 & 1**
<!--ID: 1738378824091-->

### $X + 0$

$X + 0 = X$, by **operations with 0 & 1**
<!--ID: 1738378824093-->

### $XX$

$XX = X$, by **idempotent laws**
<!--ID: 1738378824095-->

### $X + X$

$X + X = X$, by **idempotent laws**
<!--ID: 1738378824097-->

### $\overline{X}X$

$\overline{X}X = 0$, by **law of complementary**
<!--ID: 1738378824099-->

### $\overline{X} + X$

$\overline{X} + X = 1$, by **law of complementary**
<!--ID: 1738378824101-->

### $\overline{\overline{X}}$

$\overline{\overline{X}} = X$, by **involution law**
<!--ID: 1738378824103-->

### $XY$

$XY = YX$, by **commutative law**
<!--ID: 1738378824106-->

### $X + Y$

$X + Y = Y + X$, by **commutative law**
<!--ID: 1738378824108-->

### $XY + XZ$

$XY + XZ = X(Y + Z)$, by **distributive law**
<!--ID: 1738378824110-->

### $(X + Y)(X + Z)$

$(X + Y)(X + Z) = X + YZ$, by **distributive law**
<!--ID: 1738378824112-->

### $(XY)Z$

$(XY)Z = X(YZ)$, by **associative law**
<!--ID: 1738378824114-->

### $(X + Y) + Z$

$(X + Y) + Z = X + (Y + Z)$, by **associative law**
<!--ID: 1738378824116-->

### $X(X + Y)$

$X(X + Y) = X$, by **absorption**
<!--ID: 1738378824118-->

### $X + XY$

$X + XY = X$, by **absorption**
<!--ID: 1738378824120-->

### $X(\overline{X} + Y)$

$X(\overline{X} + Y) = X Y$, by **identity**
<!--ID: 1738378824122-->

### $X + \overline{X} Y$

$X + \overline{X}Y = X + Y$, by **identity**
<!--ID: 1738378824124-->

### $\overline{X Y}$

$\overline{X Y} = \overline{X} + \overline{Y}$, by **De Morgan’s law**
<!--ID: 1738378824126-->

### $\overline{X + Y}$

$\overline{X + Y} = \overline{X} \overline{Y}$, by **De Morgan’s law**
<!--ID: 1738378824128-->

### $(X + Y)(\overline{X} + Z)(Y + Z)$

$(X + Y)(\overline{X} + Z)(Y + Z) = (X + Y)(\overline{X} + Z)$, by **consensus theorem**
<!--ID: 1738378824130-->

### $X Y + \overline{X} Z + Y Z$

$X Y + \overline{X} Z + Y Z = X Y + \overline{X} Z$, by **consensus theorem**
<!--ID: 1738378824132-->

### $(X + Y)(X + \overline{Y})$

$(X + Y)(X + \overline{Y}) = X$, by **simplification theorem**
<!--ID: 1738378824135-->

### $X Y + X \overline{Y}$

$X Y + X \overline{Y} = X$, by **simplification theorem**
<!--ID: 1738378824138-->

### $(X + Y)(\overline{X} + Z)$

$(X + Y)(\overline{X} + Z) = X Z + \overline{X} Y$, by **multiplying out & factoring theorem**
<!--ID: 1738378824140-->

### $X Y + \overline{X} Z$

$X Y + \overline{X} Z = (X + Z)(\overline{X} + Y)$, by **multiplying out & factoring theorem**
<!--ID: 1738378824143-->
